Finer-grained tracking of translation units.

theories/lang/cpp/logic/dispatch.v
@@ -90,12 +90,14 @@ Section with_cpp.
   (** [resolve_virtual σ this cls f Q] returns [Q fa this'] if resolving [f] on
       [this] results in a function that is equivalent to calling the pointer [fa]
       passing [this'] as the "this" argument.
+
+      TODO: this definition should be changed to use [tu_get_impl] above.
    *)
   Definition resolve_virtual
-             (this : ptr) (cls : globname) (f : obj_name)
+             {σ : genv} (this : ptr) (cls : globname) (f : obj_name)
              (Q : forall (faddr : ptr) (cls_type : globname) (this_addr : ptr), mpred)
     : mpred :=
-    Exists (path : list globname) σ tu, denoteModule (resolve:=σ) tu **
+    Exists (path : list globname), (* denoteModule (resolve:=σ) tu ** *)
       ((Exists q, this |-> identityR cls path q ** [| path <> nil |] ** True) //\\
       match get_impl cls path f with
       | Some (fa, cls, off) => Q fa cls (_offset_ptr this off)
@@ -103,7 +105,7 @@ Section with_cpp.
         False
       end).
 
-  Lemma resolve_virtual_frame (cls : globname) (this : ptr) s
+  Lemma resolve_virtual_frame {σ : genv} (cls : globname) (this : ptr) s
     (Q Q' : ptr → globname → ptr → mpredI) :
         Forall (a : ptr) (b : globname) (c : ptr), Q a b c -* Q' a b c
     |-- resolve_virtual this cls (s_dtor s) Q -* resolve_virtual this cls (s_dtor s) Q'.
@@ -111,8 +113,8 @@ Section with_cpp.
     intros.
     rewrite /resolve_virtual.
     iIntros "X Y".
-    iDestruct "Y" as (path ? ?) "[? Y]".
-    iExists path, _, _; iFrame.
+    iDestruct "Y" as (path) "Y".
+    iExists path; iFrame.
     iSplit.
     { iDestruct "Y" as "[$ _]". }
     { iDestruct "Y" as "[_ Y]". case_match => //.
